

# Bernoulli Numbers and Polynomials

Matthew Gergley

December 18, 2025

## 1 Brief History

The Bernoulli numbers are terms of a sequence of rational numbers discovered independently by Jakob Bernoulli and Seki Takakazu. These numbers were discovered in an effort to define a general formula for the sum of integer powers,

$$\sum_{k=1}^n k^m$$

for integers  $m \geq 1$ . We do not discuss here the procedure in which Bernoulli and Takakazu each uncovered these numbers; the curious reader can seek out derivations that were followed by both renown mathematicians.

## 2 Applications

Here are just a few of the applications of Bernoulli numbers:

- Riemann-Zeta function (Number Theory)
- Kervaire-Milnor formula (Topology and Geometry)
- Quantum Harmonic Oscillator (Quantum Physics)
- Modular Forms and Elliptic Curves
- $p$ -adic Analysis and  $p$ -adic Zeta functions (Number Theory)
- Algebraic  $K$ -theory and Motivic Cohomology (Algebraic geometry and topology)

⋮

## 3 Definition/Construction of Bernoulli Numbers

One of the ways that Bernoulli numbers are defined is the following

$$F(t) = \frac{t}{e^t - 1} = \sum_{n=0}^{\infty} B_n \frac{t^n}{n!}$$

where the Bernoulli numbers are the coefficients of the power series,  $B_n$ . Hence, we derived a formula for these numbers.

We start with the exponential power series and turn it into a power series for  $\frac{t}{e^t - 1}$ . Thus,

$$e^t = \sum_{k=0}^{\infty} \frac{t^k}{k!} = 1 + t + \frac{t^2}{2} + \frac{t^3}{6} + \cdots$$

Then,

$$e^t - 1 = t + \frac{t^2}{2} + \frac{t^3}{6} + \frac{t^4}{24} + \dots$$

$$= \sum_{n=1}^{\infty} b_n t^n$$

with  $b_1 = 1$ ,  $b_2 = \frac{1}{2}$ ,  $b_3 = \frac{1}{6}$ ,  $\dots$ ,  $b_k = \frac{1}{k!}$ ,  $\dots$ . We want the following power series,

$$\frac{t}{e^t - 1} = t \cdot \left( \frac{1}{\sum_{n=1}^{\infty} b_n t^n} \right)$$

Observe in  $e^t - 1 = t \left( 1 + \frac{t}{2} + \frac{t^2}{6} + \dots \right)$  that  $1 + \frac{t}{2} + \frac{t^2}{6} + \dots \rightarrow 1$  as  $t \rightarrow 0$ . Thus, near 0,  $e^t - 1 \sim t$ . Then

$$\frac{1}{e^t - 1} \sim \frac{1}{t}$$

Therefore we need a Laurent series since  $\frac{t}{e^t - 1}$  is not analytic at 0. The coefficient of  $t^{-1}$  is called the **residue** or **pole's leading coefficient**. In this case, the residue must be 1 due to the asymptotic behavior  $\frac{1}{e^t - 1} \sim \frac{1}{t}$ . Let

$$\frac{1}{e^t - 1} = \sum_{n=-1}^{\infty} c_n t^n$$

since we expect a  $\frac{1}{t}$  pole. The first term is  $c_{-1} t^{-1}$  since the singularity is exactly a first-order pole, i.e. not  $1/t^2$ ,  $1/t^3$ , etc., we only need one negative power term. Now consider

$$1 = (e^t - 1) \left( \frac{1}{e^t - 1} \right) = \left( \sum_{k=1}^{\infty} b_k t^k \right) \left( \sum_{n=-1}^{\infty} c_n t^n \right)$$

By multiplying these power series (series convolution), the coefficient of  $t^m$  in the product is

$$\sum_{k+n=m} b_k c_n$$

Since  $\left( \sum_{k=1}^{\infty} b_k t^k \right) \left( \sum_{n=-1}^{\infty} c_n t^n \right) = 1$ , the coefficient of  $t^0$  must be 1, and the coefficient of every  $t^m$  for  $m \geq 1$  must be 0. We know what the coefficients of  $b_j$  are thus we wish to solve for the  $c_i$ . We solve a few of these below and note that  $k \geq 1$  and  $n \geq -1$  by their respective series definitions:  
( $m = 0$ ) constant term; coeff. of  $t^0$ :

$$\sum_{k+n=0} b_k c_n = 1$$

Since  $b_1 = 1 \Rightarrow c_{-1} = 1$ .

( $m = 1$ ) coeff. of  $t^1$ :

$$\sum_{k+n=1} b_k c_n = \sum_{k+n=1} b_k c_n = b_1 c_0 + b_2 c_{-1} = 0$$

Thus, since  $b_1 = 1$ ,  $b_2 = \frac{1}{2}$ ,  $c_{-1} = 1$ , we have  $c_0 = -\frac{1}{2}$ .

( $m = 2$ ) coeff. of  $t^2$ :

$$\sum_{k+n=2} b_k c_n = \sum_{k+n=2} b_k c_n = b_1 c_1 + b_2 c_0 + b_3 c_{-1} = 0$$

And thus, since  $b_1 = 1$ ,  $b_2 = \frac{1}{2}$ ,  $b_3 = \frac{1}{6}$ ,  $c_0 = -\frac{1}{2}$ ,  $c_{-1} = 1$ , we have  $c_1 = \frac{1}{12}$ .  
 Now we return back to the Laurent expansion of  $\frac{1}{e^t - 1}$  about  $t = 0$ ,

$$\sum_{n=-1}^{\infty} c_n t^n$$

and multiply by  $t$  to obtain the Taylor expansion for  $\frac{t}{e^t-1}$ :

$$\frac{t}{e^t-1} = \sum_{n=0}^{\infty} d_n t^n = \sum_{n=0}^{\infty} B_n \frac{t^n}{n!}$$

Therefore,  $d_n = c_{n-1}$ . Hence,

$$\begin{aligned} \frac{t}{e^t-1} &= c_{-1} + c_0 t + c_1 t^2 + \dots \\ &= 1 - \frac{t}{2} + \frac{t^2}{12} + \dots \end{aligned}$$

And by the series equivalence, we have  $d_n = \frac{B_n}{n!} \Rightarrow B_n = d_n n! = c_{n-1} n!$ . Thus, for example,  $B_0 = c_{-1} = 1$ ,  $B_1 = c_0 = -\frac{1}{2}$ , and  $B_2 = 2c_1 = \frac{1}{6}$ .

Therefore, we have derived an explicit way to compute Bernoulli numbers through a construction starting from the exponential series.

## 4 Definition/Construction of Bernoulli Polynomials

Define the Bernoulli polynomials,  $B_k(X)$ , by the power series expansion

$$F_f(t, X) = \frac{te^{tX}}{e^t-1} = \sum_{k=0}^{\infty} B_k(X) \frac{t^k}{k!}$$

The explicit formula for  $B_n(X)$  is

$$B_n(X) = \sum_{k=0}^n \binom{n}{k} B_{n-k} X^k \quad (1)$$

We derive this explicit formula below via the Taylor expansion,  $\frac{t}{e^t-1}$ , that we calculated in the previous section:

$$e^{tX} = \sum_{m=0}^{\infty} \frac{(tX)^m}{m!}$$

Thus,

$$\begin{aligned} \frac{te^{tX}}{e^t-1} &= \left( \frac{t}{e^t-1} \right) (e^{tX}) = \left( \sum_{k=0}^{\infty} d_k t^k \right) \left( \sum_{m=0}^{\infty} \frac{(tX)^m}{m!} \right) \\ &= \left( \sum_{k=0}^{\infty} B_k \frac{t^k}{k!} \right) \left( \sum_{m=0}^{\infty} \frac{(tX)^m}{m!} \right) \\ &= \sum_{n=0}^{\infty} \left( \sum_{k+m=n} B_k \frac{X^m}{k!m!} \right) t^n \\ &= \sum_{n=0}^{\infty} \left( \sum_{k=0}^n B_k \frac{X^{n-k}}{k!(n-k)!} \right) t^n \quad \because m = n - k \end{aligned}$$

Our goal is to get something of the form  $\sum(\text{something}) \frac{t^n}{n!}$ . Hence, multiply  $\frac{1}{k!(n-k)!}$  by  $\frac{n!}{n!} \Rightarrow \frac{1}{n!} \cdot \binom{n}{k}$ . Thus we have

$$\sum_{k=0}^n B_k \frac{X^{n-k}}{k!(n-k)!} = \frac{1}{n!} \sum_{k=0}^n \binom{n}{k} B_k X^{n-k}$$

Substituting this back into the series,

$$\begin{aligned} & \sum_{n=0}^{\infty} \left( \sum_{k=0}^n B_k \frac{X^{n-k}}{k!(n-k)!} \right) t^n \\ &= \sum_{n=0}^{\infty} \left( \frac{1}{n!} \sum_{k=0}^n \binom{n}{k} B_k X^{n-k} \right) t^n \\ &= \sum_{n=0}^{\infty} \left( \sum_{k=0}^n \binom{n}{k} B_k X^{n-k} \right) \frac{t^n}{n!} \end{aligned}$$

Thus,

$$\frac{te^{tX}}{e^t - 1} = \sum_{n=0}^{\infty} B_n(X) t^n = \sum_{n=0}^{\infty} \left( \sum_{k=0}^n \binom{n}{k} B_k X^{n-k} \right) \frac{t^n}{n!}$$

Therefore, by series equivalence,

$$B_n(X) = \sum_{k=0}^n \binom{n}{k} B_k X^{n-k} \quad (2)$$

as was to be shown (Note: Equations (1) and (2) differ only by a re-indexing of the summation; their equivalence follows by a simple change of variables). Below we calculate a few examples that demonstrate that the constant term of the  $n$ th Bernoulli polynomial is the  $n$ th Bernoulli number:

- $B_0(X) = \binom{0}{0} B_0 x^0 = B_0 = 1$
- $B_1(X) = \binom{1}{0} B_0 X^1 + \binom{1}{1} B_1 X^0 = B_0 X + B_1 = X - \frac{1}{2}$
- $B_2(X) = \binom{2}{0} B_0 X^2 + \binom{2}{1} B_1 X^1 + \binom{2}{2} B_2 X^0 = B_0 X^2 + 2B_1 X + B_2 = X^2 - X + \frac{1}{6}$